잠깐, 이제 보니, 'parent_result'가 말이 되나...??

src/study/Nemonuri.Study.CSharpSyntaxRewriter2.Modifier2/Nemonuri.StratifiedNodes.Children.fst
@@ -3,27 +3,20 @@ module Nemonuri.StratifiedNodes.Children
 module L = FStar.List.Tot
 module N = Nemonuri.StratifiedNodes.Nodes
 
-//--- propositions ---
-
-//---|
-
 //--- theory members ---
 let is_child #t (parent_node:N.node t) (node:N.node t) 
   : Pure bool (requires True) (ensures fun _ -> N.node_level_is_greater_than_levels_of_nodes_in_children t)
-    //Tot (b:bool{N.node_level_is_greater_than_levels_of_nodes_in_children t}) 
-    //if b then (N.get_level node) < (N.get_level parent_node) else true
   =
   N.lemma_node_level_is_greater_than_levels_of_nodes_in_children t;
   L.contains node (N.get_children parent_node)
+//---|
 
-(*
-  let result = (L.contains node (N.get_children parent_node)) in
-  if result then
-    (
-      N.lemma_node_level_is_greater_than_level_of_node_in_children parent_node node;
-      true
-    )
-  else
-    false
-*)
+//--- asserts ---
+let test_is_child1 = assert (
+  forall (t:eqtype) (parent_node:N.node t) (node:N.node t).
+    (is_child parent_node node) ==> (parent_node.level > node.level))
+//---|
+
+//--- propositions ---
+
 //---|
