src/study/Nemonuri.Study.CSharpSyntaxRewriter2.Modifier2/Nemonuri.StratifiedNodes.Walkers.fst
@@ -1,0 +1,37 @@
+module Nemonuri.StratifiedNodes.Walkers
+
+module L = FStar.List.Tot
+module N = Nemonuri.StratifiedNodes.Nodes
+module NC = Nemonuri.StratifiedNodes.Children
+module Option = FStar.Option
+
+//--- type definitions ---
+
+//---|
+
+//--- theory members ---
+let rec walk #t (#t_result:Type) //(#t_state:Type)
+  (node:N.node t) //(state:t_state)
+  (selector:N.node t -> t_result)
+  (aggregator:list t_result -> t_result)
+  (folder:(from_parent:t_result) -> (from_current:t_result) -> t_result)
+  (continue_predicate:t_result -> bool)
+  (parent:option (N.node t))
+  (parent_result: (option (t_result)){ (Option.isNone parent && Option.isNone parent_result) || (Option.isSome parent && Option.isSome parent_result) })
+  : Tot t_result (decreases (node.level)) =
+  if (N.is_leaf node) then (
+    let v1 = selector node in
+    match parent with
+    | None -> v1
+    | Some _ -> (
+      let Some v2 = parent_result in
+      folder v1 v2
+    )
+  ) else
+  let children = N.get_children node in
+  let results = L.map (fun child_node ->
+    walk child_node selector aggregator folder continue_predicate 
+  ) children in
+  
+    
+//---|
